add trait ready body callee helpers

rocq/theories/TypeSystem/End2EndSafety.v
@@ -12633,6 +12633,52 @@ Definition component_body_local_bounds_ready_body_summary_provider_in_env
     env_fns_root_shadow_ready_body_summary_evidence
       (global_env_with_local_bounds env (fn_bounds f_component)).
 
+Definition fn_root_shadow_summary_evidence_at
+    (env : global_env) (fname : ident) : Prop :=
+  forall fdef,
+    lookup_fn fname (env_fns env) = Some fdef ->
+    callee_body_root_shadow_summary env fdef.
+
+Definition fn_root_shadow_ready_body_summary_evidence_at
+    (env : global_env) (fname : ident) : Prop :=
+  forall fdef,
+    lookup_fn fname (env_fns env) = Some fdef ->
+    callee_body_root_shadow_synthetic_direct_call_ready_summary env fdef \/
+    callee_body_root_shadow_summary env fdef.
+
+Lemma fn_root_shadow_summary_evidence_at_of_env :
+  forall env fname,
+    env_fns_root_shadow_summary_evidence env ->
+    fn_root_shadow_summary_evidence_at env fname.
+Proof.
+  intros env fname Hsummary fdef Hlookup.
+  eapply Hsummary. exact Hlookup.
+Qed.
+
+Lemma fn_root_shadow_ready_body_summary_evidence_at_of_env :
+  forall env fname,
+    env_fns_root_shadow_ready_body_summary_evidence env ->
+    fn_root_shadow_ready_body_summary_evidence_at env fname.
+Proof.
+  intros env fname Hsummary fdef Hlookup.
+  eapply Hsummary. exact Hlookup.
+Qed.
+
+Lemma component_body_local_bounds_ready_body_summary_provider_at_in :
+  forall env,
+    component_body_local_bounds_ready_body_summary_provider_in_env env ->
+    forall f_component fname,
+      In f_component (env_fns env) ->
+      check_fn_root_shadow_no_capture_direct_call_component_store_safe_summary
+        env f_component = true ->
+      fn_root_shadow_ready_body_summary_evidence_at
+        (global_env_with_local_bounds env (fn_bounds f_component)) fname.
+Proof.
+  intros env Hprovider f_component fname Hin Hcheck.
+  eapply fn_root_shadow_ready_body_summary_evidence_at_of_env.
+  eapply Hprovider; eassumption.
+Qed.
+
 Lemma check_fn_root_shadow_synthetic_direct_call_ready_summary_sound :
   forall env fdef,
     check_fn_root_shadow_synthetic_direct_call_ready_summary env fdef =
